feat(Views) add IMP-Minus with Calls support and example

Cook_Levin_IMP/Views/IMP_Minus/Let_To_IMP_Minus_Locale.thy
@@ -1,42 +1,42 @@
 \<^marker>\<open>creator "Maximilian Schäffeler"\<close>
 \<^marker>\<open>contributor "Kevin Kappelmann"\<close>
-theory While_To_IMP_Minus_Locale
+theory Let_To_IMP_Minus_Locale
   imports IMP_Minus.Call_By_Prefixes
 begin
 
-locale While_To_IMP_Minus =
+locale Let_To_IMP_Minus =
   fixes
     cond_var :: string and
     cond_let :: \<open>'s \<Rightarrow> nat\<close> and
     cond_imp :: \<open>Com.com\<close> and
     body_let :: \<open>'s \<Rightarrow> 's\<close> and
-    body_imp :: \<open>Com.com \<close> and
+    body_imp :: \<open>Com.com\<close> and
     base_let :: \<open>'s \<Rightarrow> 's\<close> and
     base_imp :: \<open>Com.com\<close> and
-    imp_to_let_state :: \<open>string \<Rightarrow> (string \<Rightarrow> nat) \<Rightarrow> 's\<close> and
+    imp_to_let_state :: \<open>string \<Rightarrow> AExp.state \<Rightarrow> 's\<close> and
     loop_let :: \<open>'s \<Rightarrow> 's\<close> and
     vars :: \<open>string set\<close>
   assumes
     eq_on_vars[intro]: \<open>\<And>s s' p. (\<And>i. i \<in> vars \<Longrightarrow> s (add_prefix p i) = s' (add_prefix p i)) \<Longrightarrow>
       imp_to_let_state p s = imp_to_let_state p s'\<close> and
     condition_no_var: \<open>cond_var \<notin> vars\<close> and
-  
+
     base_eq: \<open>\<And>s t s' p. (invoke_subprogram p base_imp, s) \<Rightarrow>\<^bsup>t\<^esup> s' \<Longrightarrow>
       imp_to_let_state p s' = base_let (imp_to_let_state p s)\<close> and
-  
+
     body_eq: \<open>\<And>s t s' p. (invoke_subprogram p body_imp, s) \<Rightarrow>\<^bsup>t\<^esup> s' \<Longrightarrow>
       imp_to_let_state p s' = body_let (imp_to_let_state p s)\<close> and
-  
+
     cond_eq: \<open>\<And>s t s' p. (invoke_subprogram p cond_imp, s) \<Rightarrow>\<^bsup>t\<^esup> s' \<Longrightarrow>
       s' (add_prefix p cond_var) = cond_let (imp_to_let_state p s)
       \<and> imp_to_let_state p s' = imp_to_let_state p s\<close> and
-  
+
     loop_let: \<open>\<And>s. loop_let s = (if cond_let s \<noteq> 0 then loop_let (body_let s) else base_let s)\<close> and
     loop_let_induct: \<open>\<And>P s'. (\<And>s. (cond_let s \<noteq> 0 \<Longrightarrow> P (body_let s)) \<Longrightarrow> P s) \<Longrightarrow> P s'\<close>
 begin
 
-definition loop_imp where
-  "loop_imp \<equiv>
+definition while_imp where
+  "while_imp \<equiv>
   cond_imp;;
   WHILE cond_var \<noteq>0 DO (
     body_imp;;
@@ -44,15 +44,15 @@ definition loop_imp where
   );;
   base_imp"
 
-lemma imp_minus_correct:
-  assumes \<open>(invoke_subprogram p loop_imp, s) \<Rightarrow>\<^bsup>t\<^esup> s'\<close>
+lemma while_imp_correct:
+  assumes \<open>(invoke_subprogram p while_imp, s) \<Rightarrow>\<^bsup>t\<^esup> s'\<close>
   shows \<open>imp_to_let_state p s' = loop_let (imp_to_let_state p s)\<close>
   using assms
 proof (induction \<open>imp_to_let_state p s\<close> arbitrary: s s' t rule: loop_let_induct)
   case 1
   then show ?case
     apply(subst loop_let)
-    apply(simp only: loop_imp_def prefix_simps)
+    apply(simp only: while_imp_def prefix_simps)
     apply (erule Seq_tE)+
     apply (erule While_tE)
     subgoal
@@ -71,7 +71,7 @@ proof (induction \<open>imp_to_let_state p s\<close> arbitrary: s s' t rule: loo
       done
     done
   qed
-  
+
 end
 
 end
