Cook_Levin_IMP/Views/Examples/Elemof.thy
@@ -3,21 +3,21 @@ theory Elemof
   imports
     Cook_Levin_IMP.Primitives_IMP_Minus
     Cook_Levin_IMP.Compile_Nat
-    IMP_Minus_Views.While_To_IMP_Minus_Locale
-    IMP_Minus_Views.While_To_IMP_Minus_Tactics
+    IMP_Minus_Views.Let_To_IMP_Minus_Locale
+    IMP_Minus_Views.Let_To_IMP_Minus_Tactics
 begin
 
 lemma elemof_IMP_Minus_loop_body_correct_time:
   "(invoke_subprogram p elemof_IMP_loop_body, s) \<Rightarrow>\<^bsup>t\<^esup> s' \<Longrightarrow>
      t = elemof_state_upd_time 0 (elemof_imp_to_HOL_state p s)"
-  by (tactic \<open>HEADGOAL (While_To_IMP_Minus_Tactics.IMP_Minus_run_finish_tac'
+  by (tactic \<open>HEADGOAL (Let_To_IMP_Minus_Tactics.IMP_Minus_run_finish_tac'
     @{thm elemof_state_upd_time_def} @{thm elemof_IMP_loop_body_def}
     @{thm elemof_imp_to_HOL_state_def}
     [(@{thm tl_IMP_Minus_correct}, @{thm tl_imp_to_HOL_state_def})]
     @{cterm "elemof_IMP_vars"} @{cterm p}
     @{context})\<close>)
 
-interpretation A : While_To_IMP_Minus where
+interpretation A : Let_To_IMP_Minus where
   cond_var = elemof_while_cond and
   cond_let = elemof_imp_compute_loop_condition and
   body_let = elemof_state_upd and
@@ -33,7 +33,7 @@ interpretation A : While_To_IMP_Minus where
   subgoal by auto
   subgoal by (auto simp: elemof_complete_simps)
   subgoal for s t s' p
-    apply (tactic \<open>HEADGOAL (While_To_IMP_Minus_Tactics.IMP_Minus_run_finish_tac'
+    apply (tactic \<open>HEADGOAL (Let_To_IMP_Minus_Tactics.IMP_Minus_run_finish_tac'
       @{thm elemof_state_upd_def} @{thm elemof_IMP_loop_body_def}
       @{thm elemof_imp_to_HOL_state_def}
       [(@{thm tl_IMP_Minus_correct}, @{thm tl_imp_to_HOL_state_def})]
@@ -41,7 +41,7 @@ interpretation A : While_To_IMP_Minus where
       @{context})\<close>)
     done
   subgoal for s t s' p
-    apply (tactic \<open>HEADGOAL (While_To_IMP_Minus_Tactics.IMP_Minus_run_finish_tac (resolve0_tac @{thms conjI})
+    apply (tactic \<open>HEADGOAL (Let_To_IMP_Minus_Tactics.IMP_Minus_run_finish_tac (resolve0_tac @{thms conjI})
       @{thm elemof_imp_compute_loop_condition_def} @{thm elemof_IMP_init_while_cond_def}
       @{thm elemof_imp_to_HOL_state_def}
       [
