Cook_Levin_IMP/Views/IMP_Minus_Calls/Let_To_IMP_Minus_Calls_Tactics.thy
@@ -1,0 +1,30 @@
+\<^marker>\<open>creator "Kevin Kappelmann"\<close>
+theory Let_To_IMP_Minus_Calls_Tactics
+  imports
+    States_Cook_Levin_IMP_Minus_Calls
+    IMP_Minus.Call_By_Prefixes
+begin
+
+unbundle Com.no_com_syntax
+unbundle IMP_Calls.com'_syntax
+
+lemma Seq'_assoc:
+  "((IMP_Calls.Seq' p1 (IMP_Calls.Seq' p2 p3), s) \<Rightarrow>'\<^bsup>t\<^esup> s')
+    \<longleftrightarrow> ((IMP_Calls.Seq' (IMP_Calls.Seq' p1 p2) p3, s) \<Rightarrow>'\<^bsup>t\<^esup> s')"
+  by auto
+
+lemma Assign'D: "(x ::= a, s) \<Rightarrow>'\<^bsup>t\<^esup> s' \<Longrightarrow> t = 2 \<and> s' = s(x := aval a s)"
+  by auto
+
+lemma atomExp_add_prefix_empty_eq [simp]: "atomExp_add_prefix '''' e = e"
+  by (induction e) auto
+
+lemma aexp_add_prefix_empty_eq [simp]: "aexp_add_prefix '''' e = e"
+  by (induction e) auto
+
+lemma com_add_prefix_empty_eq [simp]: "com_add_prefix '''' p = p"
+  by (induction p) auto
+
+ML_file \<open>let_to_imp_minus_calls_tactics.ML\<close>
+
+end
